Debug egraph type inference. Use for some languages as a test

src/Pyrosome/Lang/SimpleUnit.v
@@ -5,10 +5,8 @@ Import ListNotations.
 Open Scope string.
 Open Scope list.
 From Utils Require Import Utils.
-From Pyrosome Require Import Theory.Core Elab.Elab Tools.Matches Lang.SimpleVSubst.
+From Pyrosome Require Import Theory.Core Elab.Elab Tools.Matches Lang.SimpleVSubst Tools.EGraph.TypeInference.
 Import Core.Notations.
-
-Require Coq.derive.Derive.
 
 Definition unit_lang_def : lang :=
   {[l/subst [value_subst]
@@ -22,9 +20,14 @@ Definition unit_lang_def : lang :=
     ]
   ]}.
 
-Derive unit_lang
-       SuchThat (elab_lang_ext value_subst unit_lang_def unit_lang)
-       As unit_wf.
+Definition unit_injectivity := [("tt", ["G"])].
+
+Definition unit_lang :=
+  Eval vm_compute in
+    (infer_lang_ext (exp_subst++value_subst) unit_lang_def
+       (unit_injectivity++exp_subst_injectivity++value_subst_injectivity)).
+
+Lemma unit_wf : elab_lang_ext value_subst unit_lang_def unit_lang.
 Proof. auto_elab. Qed.
 #[export] Hint Resolve unit_wf : elab_pfs.
 
@@ -37,8 +40,12 @@ Definition unit_eta_def :lang :=
   ] ]}.
 
 
-Derive unit_eta
-       SuchThat (elab_lang_ext (unit_lang ++ value_subst) unit_eta_def unit_eta)
-       As unit_eta_wf.
+Definition unit_eta :=
+  Eval vm_compute in
+    (infer_lang_ext (unit_lang++exp_subst++value_subst) unit_eta_def
+       (unit_injectivity++exp_subst_injectivity++value_subst_injectivity)).
+
+
+Lemma unit_eta_wf : elab_lang_ext (unit_lang ++ value_subst) unit_eta_def unit_eta.
 Proof. auto_elab. Qed.
 #[export] Hint Resolve unit_eta_wf : elab_pfs.
